Added size functions for finite sets, maps, and bags.
These are helpful for measures supporting recursive definitions and
induction schemes. The size functions have been added to the TypeBase,
with the intent that Induct, Induct_on, Cases, and Cases_on should be
applicable. (However, this has not been checked yet, so these might
not work.)

The size of a finite set is the number of elements in it, plus the
sizes of all the elements. (The size of a set with 0 as an element is
larger than that set with the zero deleted.)

The size of a finite map is the number of mapped elements, plus the
sizes of the mapped elements. Key size is ignored.

The size of a finite multiset is the number of elements in the
multiset plus the sizes of the elements. There are more extensive
orderings (e.g. the multiset order) but they aren't measures, which is
important for the way termination proofs are automated.

src/1/TypeBasePure.sml
@@ -702,42 +702,57 @@ fun tystring ty =
  in String.concat [thy,"$",name]
  end;
 
+(*---------------------------------------------------------------------------*)
+(* gamma models polymorphic functions of the form                            *)
+(*                                                                           *)
+(*  ty |-> ty_size size1 ... sizen arg = ...                                 *)
+(*                                                                           *)
+(* where arg is a term with a type having n type variables. In order to      *)
+(* synthesize the correct instance of ty_size, we have to match the types    *)
+(* of size1...sizen against the concrete types found in the instance of type *)
+(* ty. Hence the complex lead-up to matching.                                *)
+(*---------------------------------------------------------------------------*)
+
 fun typeValue (theta,gamma,undef) =
  let fun tyValue ty =
       case theta ty
        of SOME fvar => fvar
         | NONE =>
-           case gamma ty
-              of SOME f =>
-                  let val (tys,rng) = strip_fun (type_of f)
-                      val vty = last tys
-                      val sigma = match_type vty ty handle HOL_ERR _ => []
-                      val args = snd(dest_type ty)
-                  in list_mk_comb(inst sigma f, map tyValue args)
+            case gamma ty
+             of SOME f =>
+                 (let val args = snd(dest_type ty)
+                      val csizefns = map tyValue args
+                      val (tys,rng) = strip_fun (type_of f)
+                      val (gen_sizefn_tys,vty) = front_last tys
+                      val tyinst = match_type (list_mk_fun(gen_sizefn_tys,bool))
+                                              (list_mk_fun(map type_of csizefns,bool))
+                  in list_mk_comb(inst tyinst f, csizefns)
                   end handle HOL_ERR _ 
                       => (WARN "typeValue" 
                            ("Badly typed terms at type constructor "
                             ^Lib.quote (tystring ty)^". Continuing anyway.");
-                          undef ty)
+                          undef ty))
                | NONE => undef ty
  in tyValue
  end
 
-(*---------------------------------------------------------------------------
-    Map a HOL type (ty) into a term having type :ty -> num.
- ---------------------------------------------------------------------------*)
+(*---------------------------------------------------------------------------*)
+(*    Map a HOL type (ty) into a term having type :ty -> num.                *)
+(*---------------------------------------------------------------------------*)
 
 fun num() = mk_thy_type{Tyop="num",Thy="num",Args=[]}
 fun Zero() = mk_thy_const{Name="0",Thy="num", Ty=num()}
              handle HOL_ERR _ => 
              raise ERR "type_size.Zero()" "Numbers not declared"
 
-fun K0 ty = mk_abs(mk_var("v",ty),Zero())
-fun tysize_env db = Option.map fst o
-                    Option.composePartial (size_of,fetch db);
-fun theta ty = if is_vartype ty then SOME (K0 ty) else NONE
-
-fun type_size db ty = typeValue (theta,tysize_env db,K0) ty;
+fun type_size db ty = 
+ let fun K0 ty = mk_abs(mk_var("v",ty),Zero())
+     fun theta ty = if is_vartype ty then SOME (K0 ty) else NONE
+     val gamma = Option.map fst o
+                 Option.composePartial (size_of,fetch db)
+  in 
+    typeValue (theta,gamma,K0) ty
+  end
 
 (*---------------------------------------------------------------------------
     Encoding: map a HOL type (ty) into a term having type :ty -> bool list
